a more abstract cache state machine

concurrency/scache/SimpleCacheSM.i.dfy
@@ -1,78 +1,90 @@
 include "../framework/DiskSSM.s.dfy"
 include "CacheTypes.i.dfy"
+include "CacheSpec.s.dfy"
 
 module SimpleCacheStateMachine refines StateMachine(CrashAsyncIfc(CacheIfc)) {
-  import opened CacheTypes
+  import opened NativeTypes
+  import opened RequestIds
+  import CacheIfc
 
   datatype Entry =
     | Empty
     | Reading(disk_idx: nat)
-    | Full(disk_idx: nat, data: seq<byte>)
+    | Clean(disk_idx: nat, data: seq<byte>)
     | Dirty(disk_idx: nat, data: seq<byte>)
     | Writeback(disk_idx: nat, data: seq<byte>)
-  )
 
   datatype Variables = Variables(
-    entries: map<nat, Entry>,
+    entries: imap<nat, Entry>,
     write_reqs: map<nat, seq<byte>>,
     write_resps: set<nat>,
     read_reqs: set<nat>,
     read_resps: map<nat, seq<byte>>,
-    tickets: map<RequestId, IOIfc.Input>,
-    stubs: map<RequestId, IOIfc.Output>
-    disk: map<nat, seq<byte>>
+    tickets: map<RequestId, CacheIfc.Input>,
+    stubs: map<RequestId, CacheIfc.Output>,
+    disk: imap<nat, seq<byte>>
   )
 
-  predicate StartRead(s: Variables, s': Variables, op: IOIfc.Op, cache_idx: nat, disk_idx: nat) {
+  predicate Init(s: Variables) {
+    && s.entries == (imap k | true :: Empty)
+    && s.write_reqs == map[]
+    && s.write_resps == {}
+    && s.read_reqs == {}
+    && s.read_resps == map[]
+    && s.tickets == map[]
+    && s.stubs == map[]
+  }
+
+  predicate StartRead(s: Variables, s': Variables, op: ifc.Op, cache_idx: nat, disk_idx: nat) {
     && op.InternalOp?
     && cache_idx in s.entries
     && s.entries[cache_idx].Empty?
-    && (forall i | i in entries :: entries[i].status != Empty ==>
-          entries[i].disk_idx != disk_idx)
+    && (forall i | i in s.entries :: !s.entries[i].Empty? ==>
+          s.entries[i].disk_idx != disk_idx)
     && s' == s
       .(entries := s.entries[cache_idx := Reading(disk_idx)])
       .(read_reqs := s.read_reqs + {disk_idx})
   }
 
-  predicate FinishRead(s: Variables, s': Variables, op: IOIfc.Op, cache_idx: nat, disk_idx: nat) {
+  predicate FinishRead(s: Variables, s': Variables, op: ifc.Op, cache_idx: nat, disk_idx: nat) {
     && op.InternalOp?
     && cache_idx in s.entries
     && disk_idx in s.read_resps
     && s.entries[cache_idx].Reading?
     && s.entries[cache_idx].disk_idx == disk_idx
     && s' == s
-      .(entries := s.entries[cache_idx := Clean(disk_idx, s.read_resps[disk_idx].data)])
+      .(entries := s.entries[cache_idx := Clean(disk_idx, s.read_resps[disk_idx])])
       .(read_resps := s.read_resps - {disk_idx})
   }
 
-  predicate MakeDirty(s: Variables, s': Variables, op: IOIfc.Op, cache_idx: nat) {
+  predicate MakeDirty(s: Variables, s': Variables, op: ifc.Op, cache_idx: nat) {
     && op.InternalOp?
     && cache_idx in s.entries
     && s.entries[cache_idx].Clean?
-    && s' == s.(entries := s.entries[cache_idx := Dirty(s.entries[cache_idx].disk_idx, s.entries[cache_idx].data))
+    && s' == s.(entries := s.entries[cache_idx := Dirty(s.entries[cache_idx].disk_idx, s.entries[cache_idx].data)])
   }
 
-  predicate StartWriteback(s: Variables, s': Variables, op: IOIfc.Op, cache_idx: nat, disk_idx: nat) {
+  predicate StartWriteback(s: Variables, s': Variables, op: ifc.Op, cache_idx: nat, disk_idx: nat) {
     && op.InternalOp?
     && cache_idx in s.entries
     && s.entries[cache_idx].Dirty?
     && s.entries[cache_idx].disk_idx == disk_idx
     && s' == s
-        .(entries := s.entries[cache_idx] := Writeback(s.entries[cache_idx].disk_idx, s.entries[cache_idx].data))
+        .(entries := s.entries[cache_idx := Writeback(s.entries[cache_idx].disk_idx, s.entries[cache_idx].data)])
         .(write_reqs := s.write_reqs[disk_idx := s.entries[cache_idx].data])
   }
 
-  predicate FinishWriteback(s: Variables, s': Variables, op: IOIfc.Op, cache_idx: nat, disk_idx: nat) {
+  predicate FinishWriteback(s: Variables, s': Variables, op: ifc.Op, cache_idx: nat, disk_idx: nat) {
     && op.InternalOp?
     && cache_idx in s.entries
     && s.entries[cache_idx].Writeback?
     && s.entries[cache_idx].disk_idx == disk_idx
     && s' == s
-        .(entries := s.entries[cache_idx] := Clean(s.entries[cache_idx].disk_idx, s.entries[cache_idx].data))
+        .(entries := s.entries[cache_idx := Clean(s.entries[cache_idx].disk_idx, s.entries[cache_idx].data)])
         .(write_resps := s.write_resps - {disk_idx})
   }
 
-  predicate Evict(s: Variables, s': Variables, op: IOIfc.Op, cache_idx: nat) {
+  predicate Evict(s: Variables, s': Variables, op: ifc.Op, cache_idx: nat) {
     && op.InternalOp?
     && cache_idx in s.entries
     && s.entries[cache_idx].Clean?
@@ -80,7 +92,7 @@ module SimpleCacheStateMachine refines StateMachine(CrashAsyncIfc(CacheIfc)) {
         .(entries := s.entries[cache_idx := Empty])
   }
 
-  predicate ProcessRead(s: Variables, s': Variables, op: IOIfc.Op, disk_idx: nat) {
+  predicate ProcessRead(s: Variables, s': Variables, op: ifc.Op, disk_idx: nat) {
     && op.InternalOp?
     && disk_idx in s.read_reqs
     && disk_idx in s.disk
@@ -89,15 +101,102 @@ module SimpleCacheStateMachine refines StateMachine(CrashAsyncIfc(CacheIfc)) {
         .(read_resps := s.read_resps[disk_idx := s.disk[disk_idx]])
   }
 
-  predicate ProcessWrite(s: Variables, s': Variables, op: IOIfc.Op, disk_idx: nat) {
+  predicate ProcessWrite(s: Variables, s': Variables, op: ifc.Op, disk_idx: nat) {
     && op.InternalOp?
     && disk_idx in s.write_reqs
     && s' == s
         .(write_reqs := s.write_reqs - {disk_idx})
-        .(write_resps := s.write_resps[disk_idx + {disk_idx}])
-        .(disk := s.disk[disk_idx := s.write_reqs[disk_idx].data])
+        .(write_resps := s.write_resps + {disk_idx})
+        .(disk := s.disk[disk_idx := s.write_reqs[disk_idx]])
   }
 
-  predicate Crash(s: Variables, s': Variables, op: IOIfc.Op) {
+  predicate Crash(s: Variables, s': Variables, op: ifc.Op) {
+    && op.CrashOp?
+    && s'.entries == (imap k | true :: Empty)
+    && s'.write_reqs == map[]
+    && s'.write_resps == {}
+    && s'.read_reqs == {}
+    && s'.read_resps == map[]
+    && s'.tickets == map[]
+    && s'.stubs == map[]
+    && s'.disk == s.disk
+  }
+
+  predicate NewTicket(s: Variables, s': Variables, op: ifc.Op) {
+    && op.Start?
+    && op.rid !in s.tickets
+    && s' == s.(tickets := s.tickets[op.rid := op.input])
+  }
+
+  predicate ConsumeStub(s: Variables, s': Variables, op: ifc.Op) {
+    && op.End?
+    && op.rid in s.stubs && s.stubs[op.rid] == op.output
+    && s' == s.(stubs := s.stubs - {op.rid})
+  }
+
+  predicate ApplyRead(s: Variables, s': Variables, op: ifc.Op,
+      rid: RequestId, cache_idx: nat) {
+    && op.InternalOp?
+    && rid in s.tickets
+    && s.tickets[rid].ReadInput?
+    && cache_idx in s.entries
+    && (s.entries[cache_idx].Clean? || s.entries[cache_idx].Dirty?
+        || s.entries[cache_idx].Writeback?)
+    && s.entries[cache_idx].disk_idx == s.tickets[rid].key
+    && s' == s
+      .(tickets := s.tickets - {rid})
+      .(stubs := s.stubs[rid := CacheIfc.ReadOutput(s.entries[cache_idx].data)])
+  }
+
+  predicate ApplyWrite(s: Variables, s': Variables, op: ifc.Op,
+      rid: RequestId, cache_idx: nat) {
+    && op.InternalOp?
+    && rid in s.tickets
+    && s.tickets[rid].WriteInput?
+    && cache_idx in s.entries
+    && s.entries[cache_idx].Dirty? // can only write if it's marked dirty
+    && s.entries[cache_idx].disk_idx == s.tickets[rid].key
+    && s' == s
+      .(tickets := s.tickets - {rid})
+      .(stubs := s.stubs[rid := CacheIfc.WriteOutput])
+      .(entries := s.entries[cache_idx :=
+          Dirty(s.entries[cache_idx].disk_idx, s.tickets[rid].data)])
+  }
+  
+  datatype Step =
+     | StartRead_Step(cache_idx: nat, disk_idx: nat)
+     | FinishRead_Step(cache_idx: nat, disk_idx: nat) 
+     | MakeDirty_Step(cache_idx: nat) 
+     | StartWriteback_Step(cache_idx: nat, disk_idx: nat) 
+     | FinishWriteback_Step(cache_idx: nat, disk_idx: nat) 
+     | Evict_Step(cache_idx: nat) 
+     | ProcessRead_Step(disk_idx: nat) 
+     | ProcessWrite_Step(disk_idx: nat) 
+     | Crash_Step
+     | NewTicket_Step
+     | ConsumeStub_Step
+     | ApplyRead_Step(rid: RequestId, cache_idx: nat) 
+     | ApplyWrite_Step(rid: RequestId, cache_idx: nat) 
+
+  predicate NextStep(s: Variables, s': Variables, op: ifc.Op, step: Step) {
+    match step {
+       case StartRead_Step(cache_idx, disk_idx) => StartRead(s, s', op, cache_idx, disk_idx)
+       case FinishRead_Step(cache_idx, disk_idx) => FinishRead(s, s', op, cache_idx, disk_idx)
+       case MakeDirty_Step(cache_idx) => MakeDirty(s, s', op, cache_idx)
+       case StartWriteback_Step(cache_idx, disk_idx) => StartWriteback(s, s', op, cache_idx, disk_idx)
+       case FinishWriteback_Step(cache_idx, disk_idx) => FinishWriteback(s, s', op, cache_idx, disk_idx) 
+       case Evict_Step(cache_idx) => Evict(s, s', op, cache_idx)
+       case ProcessRead_Step(disk_idx) => ProcessRead(s, s', op, disk_idx)
+       case ProcessWrite_Step(disk_idx) => ProcessWrite(s, s', op, disk_idx)
+       case Crash_Step => Crash(s, s', op)
+       case NewTicket_Step => NewTicket(s, s', op)
+       case ConsumeStub_Step => ConsumeStub(s, s', op)
+       case ApplyRead_Step(rid, cache_idx) => ApplyRead(s, s', op, rid, cache_idx)
+       case ApplyWrite_Step(rid, cache_idx) => ApplyWrite(s, s', op, rid, cache_idx)
+    }
+  }
+
+  predicate Next(s: Variables, s': Variables, op: ifc.Op) {
+    exists step :: NextStep(s, s', op, step)
   }
 }
